proof/MatchSimModSem.v
@@ -193,7 +193,8 @@ Section MATCHSIMFORWARD.
       (MATCH: match_states sm_init idx0 st_src0 st_tgt0 sm0)
       (SOUND: exists su0 m_init, sound_state su0 m_init st_src0)
     ,
-      (<<PROGRESS: ModSem.is_step ms_src st_src0 -> ModSem.is_step ms_tgt st_tgt0>>)
+      (* (<<PROGRESS: ModSem.is_step ms_src st_src0 -> ModSem.is_step ms_tgt st_tgt0>>) *)
+      (<<PROGRESS: safe_modsem ms_src st_src0 -> ModSem.is_step ms_tgt st_tgt0>>)
       /\
       (<<STEPBSIM: forall
              tr st_tgt1
@@ -207,6 +208,16 @@ Section MATCHSIMFORWARD.
                /\ (<<MATCH: match_states sm_init idx1 st_src1 st_tgt1 sm1>>)
                     >>)
   .
+
+  Remark safe_modsem_is_smaller
+         st_src0
+         (NOTCALL: ~ ModSem.is_call ms_src st_src0)
+         (NOTRET: ~ ModSem.is_return ms_src st_src0)
+         (SAFE: safe_modsem ms_src st_src0)
+    :
+      ModSem.is_step ms_src st_src0
+  .
+  Proof. rr. specialize (SAFE _ (star_refl _ _ _ _)). des; ss. eauto. Qed.
 
   Hypothesis STEPSIM: STEPFSIM \/ STEPBSIM.
 
